commit

AP/AP/Determinacy.lean
@@ -26,9 +26,9 @@ instance {sa} [ha : AState sa] {st : Strat} [hst : st.WF] {n} :
 AState (sys.simulate st.f sa # n * 2).1 := ha.of_simulate_mul_two
 
 theorem AState.a_wins_of_ind {sa} [ha : AState sa]
-{st : Strat} [hst : st.WF] {p : State → Prop}
+{st : Strat} [hst : st.WF] {p : State → Prop} (hp : p sa)
 (h : ∀ {sa} [AState sa], p sa → ∃ sd, sys.tr sa (st.a.f sa) = some sd ∧
-∀ sa', sys.tr sd (st.d.f sd) = some sa' → p sa') (hp : p sa) :
+∀ sa', sys.tr sd (st.d.f sd) = some sa' → p sa') :
 sa.a_wins st := by
   rw [sa.a_wins_iff_mul_two]
   intro n
@@ -52,73 +52,141 @@ sa.a_wins st := by
   simp [h₃]
   exact h₂ _ h₃
 
-def aOptimalCnd (sa : State) (pa : PointZ) : Prop :=
-  ∃ sd, sys.tr sa pa = some sd ∧ ∀ pd sa', sys.tr sd pd = some sa' → sa'.a_hws
-
-open Classical in noncomputable
-def aOptimal : AStrat :=
-  .mk # λ sa => if ∃ pa, aOptimalCnd sa pa
-  then Classical.epsilon # aOptimalCnd sa
-  else Classical.epsilon # sys.validTr sa
-
-theorem wf_aOptimal : aOptimal.WF := by
-  rw [aStrat_wf_iff]
-  intro sa hsa h₁
-  dsimp [aOptimal]
-  generalize hp : Classical.epsilon (aOptimalCnd sa) = pa
-  simp
-  split_ifs with h₂
-  rotate_left
-  · have h₃ := Classical.epsilon_spec h₁
-    simp at h₃
-    exact h₃
-  simp at h₁
-  have h₃ := Classical.epsilon_spec h₂
-  rw [hp] at h₃
-  simp [aOptimalCnd] at h₃
-  exact h₃.1
-
-instance : aOptimal.WF := wf_aOptimal
-
--- #check 0 #exit
-
-theorem AState.of_ind {sa sa'} [hs : AState sa] [hs' : AState sa] {p : State → Prop}
+theorem AState.ind {sa sa'} [ha : AState sa] [ha' : AState sa'] {p : State → Prop}
 (h₁ : p sa) (h₂ : ∀ sa [AState sa] pa sd pd sa',
 sys.tr sa pa = some sd → sys.tr sd pd = some sa' → p sa')
 (h₃ : sys.Reachable sa sa') : p sa' := by
-  sorry
+  replace h₃ := System.exi_trs_of_reachable h₃
+  obtain ⟨ts, h₃⟩ := h₃
+  generalize hn : ts.length = n
+  induction n using Nat.strong_induction_on generalizing ts sa
+  nm n ih
+  cases ts; simp at h₃; simpa [←h₃]; nm pa ts
+  simp at h₃; split at h₃; simp at h₃
+  nm x sd h₄; clear x
+  have hd := DState.of_tr h₄
+  cases ts; simp at h₃; simp [h₃] at hd; nm pd ts
+  simp at h₃; split at h₃; simp at h₃
+  nm x sa₁ h₅; clear x
+  simp [add_assoc] at hn; subst hn
+  have ha₁ := AState.of_tr h₅
+  exact @ih ts.length (by simp) sa₁ _
+    (h₂ sa pa sd pd sa₁ h₄ h₅) ts h₃ rfl
 
--- #check 0 #exit
+noncomputable
+def mk_strat_fn (f : State → Option PointZ) : State → PointZ :=
+  λ s => (Option.getD · (Classical.epsilon # sys.validTr s)) # do
+    let p ← f s
+    guard # sys.validTr s p
+    return p
 
-theorem AState.a_hws_of_ind {sa : State} [hs : AState sa] {p : State → Prop}
+instance {f} : sys.SimFn # mk_strat_fn f := by
+  constructor; intro s hs h; unfold mk_strat_fn
+  have h₁ := Classical.epsilon_spec h; dsimp; cases h₂ : f s; simpa
+  nm s'; simp [guard]; split_ifs with h₃; simpa; simpa
+
+@[simp] noncomputable
+def AStrat.mk' (f : State → Option PointZ) : AStrat := ⟨mk_strat_fn f⟩
+
+@[simp] noncomputable
+def DStrat.mk' (f : State → Option PointZ) : DStrat := ⟨mk_strat_fn f⟩
+
+instance {f} : (AStrat.mk' f).WF := by simp; infer_instance
+instance {f} : (DStrat.mk' f).WF := by simp; infer_instance
+
+@[simp] theorem AStrat.f_mk {f} : (AStrat.mk f).f = f := rfl
+@[simp] theorem DStrat.f_mk {f} : (DStrat.mk f).f = f := rfl
+
+def aOptimalCnd (p : State → Prop) (sa : State) (pa : PointZ) : Prop :=
+  ∃ sd, sys.tr sa pa = some sd ∧ ∀ pd sa', sys.tr sd pd = some sa' → p sa'
+
+open Classical in noncomputable
+def aOptimal (p : State → Prop) : AStrat :=
+  .mk' # λ sa => choose? # aOptimalCnd p sa
+
+theorem wf_aOptimal {p} : (aOptimal p).WF := by
+  unfold aOptimal; infer_instance
+
+instance {p} : (aOptimal p).WF := wf_aOptimal
+
+theorem AState.a_hws_of_ind {sa : State} [ha : AState sa] {p : State → Prop}
 (h₁ : p sa) (h₂ : ∀ sa [AState sa], p sa → ∃ pa sd, sys.tr sa pa = some sd ∧
 ∀ pd sa', sys.tr sd pd = some sa' → p sa') : sa.a_hws := by
   classical
-  use aOptimal, inferInstance
+  use aOptimal p, inferInstance
   intro d hd
-  intro n
-  induction n generalizing sa p; simp
-  nm n ih
-  have h₄ := ih h₁ h₂
-  rw [System.simulate_add]
-  simp [h₄]
-  generalize h₃ : sys.simulate (Strat.mk aOptimal d).f sa n = r at h₄ ⊢
-  rcases r with ⟨sa', r⟩
-  dsimp at h₄ ⊢
-  subst h₄
-  sorry
+  apply ha.a_wins_of_ind h₁
+  clear! sa
+  intro sa ha hp
+  specialize h₂ sa hp
+  simp only [aOptimal, choose?_eq_ite]
+  replace h₂ : ∃ pa, aOptimalCnd p sa pa := h₂
+  have h₃ := Classical.epsilon_spec h₂
+  generalize h₁ : Classical.epsilon (aOptimalCnd p sa) = pa at h₃ ⊢
+  unfold aOptimalCnd at h₃
+  obtain ⟨sd, h₃, h₄⟩ := h₃; use sd
+  simp [-sys_tr_eq_some_iff, -validTr_iff, mk_strat_fn, h₂, h₁,
+    System.validTr_iff_isSome, h₃]; apply h₄
+
+theorem hist_eq_of_tr_eq_some {s s' p}
+(h : sys.tr s p = some s') : s'.hist = p :: s.hist := by
+  simp [sys, State.move] at h
+  split_ifs at h with h₁ <;> simp at h <;> obtain ⟨s', h, rfl⟩ := h <;> rfl
+
+@[simp]
+theorem hist_trs {s ps} [hs : sys.WF s] : (sys.trs s ps).1.hist =
+(ps.take # ps.length - (sys.trs s ps).2.length).reverse ++ s.hist := by
+  induction ps generalizing s; rfl
+  nm p ps ih
+  simp
+  split; simp
+  nm x s' h₁; clear x
+  have hs' := System.wf_of_tr h₁
+  rw [ih]; clear ih
+  replace h₁ := hist_eq_of_tr_eq_some h₁
+  rw [h₁, List.append_cons, ←List.reverse_cons]; clear h₁
+  generalize hn : (sys.trs s' ps).2.length = n
+  have h₁ : n ≤ ps.length; subst hn; exact System.trs_snd_length_le
+  rw [Nat.sub_add_comm h₁]; simp
+
+instance {s} [hs : sys.WF s] : sys.Tree s := by
+  rw [System.tree_iff_full_trs]
+  use hs; intro ts₁ ts₂ s' h₁ h₂
+  have h₃ := congrArg (·.1.hist) h₁
+  have h₄ := congrArg (·.1.hist) h₂
+  simp at h₃ h₄
+  simp [h₂] at h₄
+  simp [h₁, ←h₄] at h₃
+  exact h₃
+
+def getMoveFromHist (s_target s : State) : List PointZ → Option PointZ
+| [] => none
+| p :: ps => if s = s_target then some p else do
+  let s' ← sys.tr s p
+  getMoveFromHist s_target s' ps
+
+def State.getMoveAt (s s_target : State) : Option PointZ :=
+  getMoveFromHist s_target (initState s.pw) s.hist
+
+noncomputable
+def dOptimal (sa : State) : DStrat := .mk' # λ sd => do
+  let pa ← sd.getMoveAt sa
+  let sd' ← sys.tr sa pa
+  none
 
 #check 0 #exit
 
-theorem State.a_hws_of_ind {s : State} [hs : s.WF] {p : State → Prop}
-(h₁ : p s)
-(h₂ : ∀ s [s.WF], )
+theorem AState.a_hws_of_not_d_hws {sa} [ha : AState sa] (h : ¬sa.d_hws) : sa.a_hws := by
+  apply ha.a_hws_of_ind (p := (¬·.d_hws)) h; clear! sa
+  intro sa ha h
+  unfold State.d_hws at h ⊢
+  contrapose h
+  push_neg at h ⊢
 
 #check 0 #exit
 
 theorem State.a_hws_of_not_d_hws {s : State} [hs : s.WF] (h : ¬s.d_hws) : s.a_hws := by
-  simp [d_hws] at h
-  simp [a_hws]
+  unfold d_hws at h; push_neg at h
 
 #check 0 #exit
 
