AP/System/Invariant.lean
@@ -17,7 +17,7 @@ theorem invariant {p : S → Prop} {a b}
 theorem invariant_init {p : S → Prop} {a}
 (h₁ : sys.WF a) (h₂ : ∀ {a}, sys.Initial a → p a)
 (h₃ : ∀ {x y t}, p x → sys.tr x t = some y → p y) : p a := by
-  rw [wf_iff] at h₁
+  rw [wf_def] at h₁
   obtain ⟨s₀, h₁, h₄⟩ := h₁
   exact invariant (h₂ h₁) h₄ h₃
 
