AP/Util/Nat.lean
@@ -337,11 +337,14 @@ Nat.find h₁ ≤ Nat.find h₂ := by
   apply Nat.find_le; apply h₃; exact Nat.find_spec h₂
 
 @[simp]
-theorem le_self_mul_iff {a b : ℕ} :
-a ≤ a * b ↔ a = 0 ∨ b ≠ 0 := by
+theorem le_self_mul_iff {a b : ℕ} : a ≤ a * b ↔ a = 0 ∨ b ≠ 0 := by
   constructor
   · intro h; rw [or_iff_not_imp_left]
     rintro h₁ rfl; simp at h; contradiction
   rintro (rfl | h); simp
   cases b; simp at h; nm b
   simp [mul_succ]
+
+@[simp]
+theorem lt_self_add_iff {a b : ℕ} : a < a + b ↔ 0 < b :=
+  Nat.lt_add_right_iff_pos
